Finish porting generic soundness.

theories/OGS/Adequacy.v
@@ -12,117 +12,96 @@ we prove this fact by proving that these equations are eventually
 guarded in [OGS/CompGuarded.v].
 |*)
 
-From Coinduction Require Import coinduction tactics.
+(* for some reason we need this for some instance resolution *)
+From Coinduction Require Import coinduction.
 
 From OGS Require Import Prelude.
-From OGS.Utils Require Import Ctx Rel.
-From OGS.OGS Require Import Subst Obs Machine Game Strategy CompGuarded.
+From OGS.Utils Require Import Rel.
+From OGS.Ctx Require Import All Ctx.
+From OGS.OGS Require Import Subst Obs Machine Strategy CompGuarded.
 From OGS.ITree Require Import Event ITree Eq Delay Structure Properties Guarded.
 
-Open Scope ctx_scope.
-
-Section withFam.
-
+Section with_param.
 (*|
-We consider a language abstractly captured as a machine
+We consider a language abstractly captured as a machine satisfying an
+appropriate axiomatization.
 |*)
-  Context {bT : baseT}.
-  Context {bV : baseV}.
-  Context {bC : baseC}.
-  Context {sV : subst_monoid bV}.
-  Context {sC : subst_module bV bC}.
-  Context {oS : observation_structure}.
-  Context {M: machine}.
-(*|
-Satisfying an appropriate axiomatization
-|*)
-  Context {sVL: subst_monoid_laws}.
-  Context {sCL: subst_module_laws}.
-  Context {VA : var_assumptions} .
-  Context {ML: machine_laws}.
+  Context {T C} {CC : context T C} {CL : context_laws T C}.
+  Context {val} {VM : subst_monoid val} {VML : subst_monoid_laws val}.
+  Context {conf} {CM : subst_module val conf} {CML : subst_module_laws val conf}.
+  Context {obs : obs_struct T C} {M : machine val conf obs} {ML : machine_laws val conf obs}.
+  Context {VV : var_assumptions val}.
 
+  (*
 (*|
 Evaluate a configuration inside an environment (assignment), returning only the message part (the "positive" or "static" part).
 |*)
-  Definition eval_in_env {Γ Δ} (e : Γ ⇒ᵥ Δ) (t : conf Γ) : delay (obs∙ Δ) :=
-    eval_to_obs (e ⊛ₜ t) .
+  Definition eval_in_env {Γ Δ} (e : Γ =[val]> Δ) (c : conf Γ) : delay (obs∙ Δ) :=
+    evalₒ (c ₜ⊛ t) .
 
   #[global] Instance eval_in_env_proper {Γ Δ} : Proper (ass_eq Γ Δ ==> eq ==> eq) (@eval_in_env Γ Δ).
     intros ? ? H1 ? ? H2; unfold eval_in_env; now rewrite H1, H2.
   Qed.
+*)
 
-  Equations reduce {Δ} : reduce_t Δ -> delay (obs∙ Δ) :=
-    reduce u := eval_in_env
-                  ([ v_var , concat1 _ (snd (fst (projT2 u))) (snd (projT2 u)) ])
-                  (fst (fst (projT2 u))) .
+  Definition reduce {Δ} (x : reduce_t Δ)
+    : delay (obs∙ Δ)
+    := evalₒ (x.(red_act).(ms_conf)
+              ₜ⊛ [ a_id , bicollapse x.(red_act).(ms_env) x.(red_pas) ]) .
 
-  Definition reduce' {Δ} : forall i, reduce_t Δ -> itree ∅ₑ (fun _ : T1 => obs∙ Δ) i := fun 'T1_0 => reduce .
+  Definition reduce' {Δ} : forall i, reduce_t Δ -> itree ∅ₑ (fun _ : T1 => obs∙ Δ) i
+    := fun 'T1_0 => reduce .
 
-  Tactic Notation "mytransitivity" := first [eapply @transitivity; [eapply it_eq_t_trans; fail | |] | etransitivity].
+  Check (it_eq_t_trans).
+
+  (*Tactic Notation "mytransitivity" := first [eapply @transitivity; [eapply it_eq_t_trans; fail | |] | etransitivity].*)
 
 (*|
 Equipped with eventually guarded equations, we are ready to prove the adequacy
 |*)
-  Lemma adequacy_pre {Δ} (x : reduce_t Δ) :
+  Lemma compo_reduce_simpl {Δ} (x : reduce_t Δ) :
     (compo_body x >>= fun _ r =>
          match r with
-         | inl x' => reduce' _ x'
-         | inr y => Ret' (y : (fun _ => obs∙ _) _)
+         | inl y => reduce' _ y
+         | inr o => Ret' (o : (fun _ => obs∙ _) _)
          end)
       ≊
-      (eval (fst (fst (projT2 x))) >>= fun _ u =>
-           match cat_split (nf'_var u) with
-           | CLeftV h => Ret' (_ ,' (h, nf'_obs u))
-           | CRightV h => reduce' _ (_ ,' (m_strat_resp (snd (projT2 x)) (_ ,' (h, nf'_obs u)) ,
-                                           snd (fst (projT2 x)) ▶ₑ⁻ nf'_val u))
+      (eval x.(red_act).(ms_conf) >>= fun _ n =>
+           match c_view_cat (nf_var n) with
+           | Vcat_l i => Ret' (i ⋅ nf_obs n)
+           | Vcat_r j => reduce' _ (RedT (m_strat_resp x.(red_pas) (j ⋅ nf_obs n))
+                                        (x.(red_act).(ms_env) ;⁻ nf_args n))
            end).
   Proof.
-    mytransitivity; [ now apply bind_bind_com | ].
-    mytransitivity; [ now apply fmap_bind_com | ].
-    unfold m_strat_play, m_strat_wrap.
-    remember (eval (fst (fst (projT2 x)))) as t eqn:H; clear H; revert t.
-    unfold it_eq; coinduction R CIH; intros t.
-    cbn; destruct (t.(_observe)) as [ [ ? [ i [ ? ? ] ] ] | | [] ]; cbn.
-    + destruct (cat_split i).
-      * econstructor; reflexivity.
-      * cbn -[eval_in_env] .
-        change (it_eqF _ _ _ _ (_observe ?a) (_observe ?b))
-          with (it_eq_map  ∅ₑ (eqᵢ _) (it_eq_t _ (eqᵢ _) R) T1_0 a b).
-        reflexivity.
-    + econstructor; apply CIH.
+    do 2 (etransitivity; [ now apply fmap_bind_com | ]).
+    apply (subst_eq (RX := fun _ => eq)); eauto.
+    intros ? [ ? i [ ? ? ] ] ? <-.
+    unfold m_strat_wrap; cbn.
+    now destruct (c_view_cat i).
   Qed.
 
-  Definition split_sub_eval {Γ Δ} (c : conf (Δ +▶ Γ)) (e : Γ ⇒ᵥ Δ) : delay (nf∙ Δ) :=
-    eval ([ v_var , e ] ⊛ₜ c) .
+  Definition eval_split_sub {Γ Δ} (c : conf (Δ +▶ Γ)) (e : Γ =[val]> Δ)
+    : delay (nf obs val Δ)
+    := eval c >>= fun 'T1_0 n =>
+         match c_view_cat (nf_var n) with
+         | Vcat_l i => Ret' (i ⋅ nf_obs n ⦇ nf_args n ⊛ [ v_var,  e ] ⦈)
+         | Vcat_r j => eval (e _ j ⊙ nf_obs n ⦗ nf_args n ⊛ [ v_var,  e ] ⦘)
+         end .
 
-  Definition eval_split_sub {Γ Δ} (c : conf (Δ +▶ Γ)) (e : Γ ⇒ᵥ Δ) : delay (nf' Δ) :=
-    eval c >>= fun 'T1_0 u =>
-        match cat_split (nf'_var u) with
-        | CLeftV h => Ret' (nf'_ty u ,' (h , (nf'_obs u ,' [ v_var,  e ] ⊛ nf'_val u)))
-        | CRightV h => eval (app (e _ h) (nf'_obs u) ([v_var , e ] ⊛ nf'_val u))
-        end .
-
-  Lemma eval_split {Γ Δ} (c : conf (Δ +▶ Γ)) (e : Γ ⇒ᵥ Δ) :
-    split_sub_eval c e ≋ eval_split_sub c e .
+  Lemma eval_split {Γ Δ} (c : conf (Δ +▶ Γ)) (e : Γ =[val]> Δ) :
+    eval (c ₜ⊛ [ a_id , e ]) ≋ eval_split_sub c e .
   Proof.
-    unfold split_sub_eval, eval_split_sub.
+    unfold eval_split_sub.
     rewrite (eval_sub c ([ v_var , e ])).
-    unfold bind_delay'.
-    remember (eval c) as t; clear c Heqt.
-    revert t; unfold comp_eq,it_eq; coinduction R CIH; cbn; intro t.
-    destruct (_observe t); [ | econstructor; apply CIH | inversion q ].
-    destruct r as [ x [ i [ m γ ] ] ]; cbn in *.
-    destruct (cat_split i).
-    + change (?u x (r_cover_l cover_cat x i)) with ((u ⊛ᵣ r_concat_l) x i).
-      rewrite s_eq_cat_l.
-      eassert (H : _) by exact (eval_nf_ret (x ,' (i , (m ,' ([v_var, e]) ⊛ γ)))).
-      unfold comp_eq in H.
-      apply it_eq_step in H; cbn in *; unfold observe in H.
-      destruct (_observe (eval (app (v_var x i) m (([v_var, e]) ⊛ γ)))); dependent elimination H; auto.
-    + change (?u x (r_cover_r cover_cat x j)) with ((u ⊛ᵣ r_concat_r) x j).
-      rewrite s_eq_cat_r.
-      destruct (_observe (eval (app (e x j) m (([v_var, e]) ⊛ γ)))); econstructor; auto.
-      now apply nf_eq_rfl'.
+    apply (subst_eq (RX := fun _ => eq)); eauto.
+    intros [] [ ? i [ o a ] ] ? <-; unfold emb; cbn.
+    destruct (c_view_cat i).
+    + unfold nf_args, fill_args, cut_r.
+      rewrite app_sub, v_sub_var.
+      cbn; rewrite c_view_cat_simpl_l.
+      now apply (eval_nf_ret (i ⋅ o ⦇ a ⊛ [a_id, e] ⦈)).
+    + rewrite app_sub, v_sub_var.
+      cbn; now rewrite c_view_cat_simpl_r.
   Qed.
 
 (*|
@@ -133,116 +112,56 @@ guarded equations.
 |*)
 
   Lemma adequacy_gen {Δ a} (c : m_strat_act Δ a) (e : m_strat_pas Δ a) :
-    reduce (_ ,' (c , e)) ≊ (c ∥g e).
+    reduce (RedT c e) ≊ (c ∥g e).
   Proof.
     refine (iter_evg_uniq (fun 'T1_0 u => compo_body u) (fun 'T1_0 u => reduce u) _ _ T1_0 _).
     clear a c e; intros [] [ ? [ u v ] ].
-    etransitivity; [ | symmetry; apply adequacy_pre ].
-    unfold reduce at 1.
-    etransitivity; [ apply eval_to_obs_eq, eval_split | ].
+    etransitivity; [ | symmetry; apply compo_reduce_simpl ].
+    unfold reduce at 1, evalₒ at 1; rewrite eval_split.
     etransitivity; [ apply bind_fmap_com | ].
-    unfold it_eq; cbn [fst snd projT2 projT1].
-    apply (tt_t (it_eq_map ∅ₑ (eqᵢ _))).
-    refine (it_eq_up2bind_t _ _ _ _ (eval (fst u) >>= _) (eval (fst u) >>= _) _); econstructor; eauto.
-    intros [] [ t1 [ i1 [ m1 γ1 ] ]] [ t2 [ i2 [ m2 γ2 ] ]] [ p [ q r ] ].
-    cbn in *.
-    revert i1 m1 γ1 q r; rewrite p; clear p t1; intros i1 m1 γ1 q r; cbn in q,r.
-    rewrite q; clear q i1.
-    destruct r as [ p q ]; cbn in p,q.
-    revert γ1 q; rewrite p; clear p m1; intros γ1 q; cbn in q.
-    apply (bt_t (it_eq_map ∅ₑ (eqᵢ (fun _ : T1 => obs∙ Δ)))).
-    pose (xx := cat_split i2); change (cat_split i2) with xx; destruct xx.
-    - cbn; econstructor; reflexivity.
-    - cbn -[it_eq_map fmap].
-      change (it_eq_t ∅ₑ (eqᵢ (fun _ : T1 => obs∙ Δ)) bot) with (it_eq (E:=∅ₑ) (eqᵢ (fun _ : T1 => obs∙ Δ))).
-      apply it_eq_step, (fmap_eq (RX := eqᵢ _)).
-      intros ? ? ? ->; auto.
-      unfold m_strat_resp; cbn [fst snd projT1 projT2].
-      rewrite app_sub, concat1_equation_2.
+    apply (subst_eq (RX := fun _ => eq)); eauto.
+    intros [] [ ? i [ o a ] ] ? <-; unfold emb; cbn.
+    destruct (c_view_cat i).
+    - rewrite c_view_cat_simpl_l.
+      apply it_eq_unstep; cbn; do 2 econstructor.
+    - rewrite c_view_cat_simpl_r.
+      unfold reduce; cbn; unfold nf_args, cut_r, fill_args; cbn.
+      assert (H : (bicollapse v red_pas cut_ty j ⊙ o ⦗ a ⊛ [a_id, bicollapse v red_pas] ⦘)
+                  = ((ₐ↓ red_pas cut_ty j ᵥ⊛ r_emb r_cat3_1) ⊙ o ⦗ r_cat_rr ᵣ⊛ a_id ⦘
+       ₜ⊛ [a_id, [bicollapse v red_pas, a ⊛ [a_id, bicollapse v red_pas]]])).             
+        rewrite app_sub, <- v_sub_sub.
+      
+        (* AAAAA setoid rewriting!!!! *)
+        etransitivity; cycle 1.
+        unshelve erewrite v_sub_proper.
+        5: { rewrite (a_ren_r_simpl _ r_cat3_1 _).
+             now rewrite r_cat3_1_simpl; eauto.
+           }
+        3,4: reflexivity.
 
-      pose (xx := [ v_var , [concat1 _ v (snd u), ([v_var, concat1 _ (snd u) v]) ⊛ γ2]] ⊛ᵥ r_concat3_1 ᵣ⊛ᵥ concat0 v t2 j).
-      change ([ v_var , [ _ , _ ]] ⊛ᵥ _) with xx.
-      assert (H : xx = concat1 _ (snd u) v t2 j); [ | rewrite H; clear H ].
-      + unfold xx; clear xx.
-        change (?a ⊛ᵥ ?b ᵣ⊛ᵥ (concat0 v _ j)) with ((a ⊛ (b ᵣ⊛ concat0 v)) _ j).
-        unfold e_ren; rewrite v_sub_sub.
-        etransitivity; [ | now apply (proj2 (concat_fixpoint (snd u) v)) ].
-        eapply e_comp_proper; [ | reflexivity ].
-        rewrite e_comp_ren_r, v_sub_var.
-        unfold r_concat3_1.
-        etransitivity; [ unfold s_ren at 1; apply s_eq_cover_map | ].
-        change (s_map ?a ?b) with (s_ren a b); change (s_cover cover_cat ?a ?b) with ([ a , b ]).
-        now rewrite s_eq_cat_l, s_ren_comp, s_eq_cat_r, s_eq_cat_l.
-      + erewrite app_proper; [ reflexivity | ].
-        now rewrite q, 2 e_comp_ren_r, v_sub_var, 2 s_eq_cat_r.
+        change (?r ᵣ⊛ a_id)%asgn with (r_emb r); rewrite a_ren_r_simpl.
+        unfold r_cat_rr; rewrite a_ren_l_comp.
+        rewrite 2 a_cat_proj_r.
+
+        pose proof (H := collapse_fix_pas v red_pas _ j).
+        cbn in H; now rewrite H.
+        exact _.
+
+      pose (xx := bicollapse v red_pas cut_ty j ⊙ o ⦗ a ⊛ [a_id, bicollapse v red_pas] ⦘).
+      change (bicollapse v _ _ _ ⊙ o ⦗ _ ⦘) with xx in H |- *.
+      now rewrite H.
   Qed.
 
 (*|
 Adequacy (Def 6.1) holds
-
-Note: Something in the refactoring broke all rewrites in this specific proof,
-there seems to be a unification problem diverging during TC search.
-To be fixed, for now we painfully fix the proofs by hand.
 |*)
-  Lemma adequacy {Γ Δ} (c : conf Γ) (e : Γ ⇒ᵥ Δ) :
-    eval_in_env e c ≊ (inj_init_act Δ c ∥g inj_init_pas e).
+  Lemma adequacy {Γ Δ} (c : conf Γ) (e : Γ =[val]> Δ) :
+    evalₒ (c ₜ⊛ e) ≊ (inj_init_act Δ c ∥g inj_init_pas e).
   Proof.
-    etransitivity; [ | apply adequacy_gen ].
-    unfold reduce, inj_init_act, eval_in_env; cbn [fst snd projT1 projT2]; apply (fmap_eq (RX:=eqᵢ _)).
-    intros ? ? ? ->; auto.
-    unfold inj_init_pas; rewrite concat1_equation_2, 2 concat1_equation_1.
-    unfold c_ren; rewrite c_sub_sub, c_sub_proper ; try reflexivity.
-    etransitivity.
-    2:{
-      eapply e_comp_proper; [| reflexivity].
-      eapply s_cover_proper; [reflexivity |].
-      eapply s_cover_proper; [reflexivity |].
-      eapply e_comp_proper; [| reflexivity].
-      apply s_eq_cover_empty_r.
-    }
-    rewrite e_comp_ren_r, v_sub_var.
-    rewrite s_ren_comp.
-    (* rewrite s_eq_cat_r. *)
-    etransitivity.
-    2:{
-      eapply s_ren_proper; [| reflexivity].
-      symmetry; apply s_eq_cat_r.
-    }
-    etransitivity.
-    2:{
-      symmetry; apply s_eq_cat_r.
-    }
-    unfold e_ren, r_concat_l, cover_cat; cbn.
-    etransitivity.
-    2:{
-      eapply e_comp_proper; [reflexivity |].
-      eapply e_comp_proper; [| reflexivity].
-      eapply s_ren_proper; [reflexivity |].
-      symmetry; apply r_cover_l_nil.
-    }
-    etransitivity.
-    2:{
-      eapply e_comp_proper; [reflexivity |].
-      eapply e_comp_proper; [| reflexivity].
-      symmetry; apply s_ren_id.
-    }
-    etransitivity.
-    2:{
-      eapply e_comp_proper; [reflexivity |].
-      symmetry; apply v_var_sub.
-    }
-    etransitivity.
-    2:{
-      eapply e_comp_proper; [| reflexivity].
-      symmetry; apply s_eq_cover_empty_r.
-    }
-    etransitivity.
-    2:{
-      eapply e_comp_proper; [| reflexivity].
-      symmetry; apply s_eq_cover_empty_r.
-    }
-    symmetry; apply v_var_sub.
+    rewrite <- adequacy_gen; unfold reduce; cbn.
+    now rewrite <- c_sub_sub, a_ren_r_simpl,
+          a_ren_l_comp, 2 a_cat_proj_r,
+          a_ren_comp, a_cat_proj_l, a_comp_id.
   Qed.
-
-End withFam.
+End with_param.
 
