theories/OGS/Soundness.v
@@ -11,65 +11,50 @@ At the end of the file, we run two commands:
 - [Print Assumptions ogs_correction.] explicit if any axiom has been used to establish the result. As stated in the Readme, we exclusively use [Eqdep.Eq_rect_eq.eq_rect_eq] (i.e., axiom K).
 |*)
 
-From Coinduction Require Import coinduction tactics.
+From Coinduction Require Import coinduction.
 
 From OGS Require Import Prelude.
-From OGS.Utils Require Import Ctx Rel.
+From OGS.Ctx Require Import All.
 From OGS.OGS Require Export Subst Obs Machine Game Strategy CompGuarded Adequacy Congruence.
-From OGS.ITree Require Import Event ITree Eq Delay Structure Properties Guarded.
+From OGS.ITree Require Import Eq Guarded.
 
-Open Scope ctx_scope.
-
-Section withFam.
-
+Section with_param.
 (*|
-We consider a language abstractly captured as a machine
+We consider a language abstractly captured as a machine satisfying an
+appropriate axiomatization.
 |*)
-  Context {bT : baseT}.
-  Context {bV : baseV}.
-  Context {bC : baseC}.
-  Context {sV : subst_monoid bV}.
-  Context {sC : subst_module bV bC}.
-  Context {oS : observation_structure}.
-  Context {M: machine}.
-(*|
-Satisfying an appropriate axiomatization
-|*)
-  Context {sVL: subst_monoid_laws}.
-  Context {sCL: subst_module_laws}.
-  Context {VA : var_assumptions} .
-  Context {ML: machine_laws}.
+  Context {T C} {CC : context T C} {CL : context_laws T C}.
+  Context {val} {VM : subst_monoid val} {VML : subst_monoid_laws val}.
+  Context {conf} {CM : subst_module val conf} {CML : subst_module_laws val conf}.
+  Context {obs : obs_struct T C} {M : machine val conf obs} {ML : machine_laws val conf obs}.
+  Context {VV : var_assumptions val}.
 
 (*|
 Substitution equivalence of two abstract machine configurations (Def 4.21)
 |*)
-  Definition ciu {Γ} Δ (x y : conf Γ) : Prop
-    := forall e : Γ ⇒ᵥ Δ, eval_in_env e x ≈ eval_in_env e y.
+  Definition ciu {Γ} Δ (a b : conf Γ) : Prop
+    := forall γ : Γ =[val]> Δ, evalₒ (a ₜ⊛ γ) ≈ evalₒ (b ₜ⊛ γ).
   Notation "x ≈⟦ciu Δ ⟧≈ y" := (ciu Δ x y) (at level 50).
 
   Definition barb {Γ} Δ (x y : conf Γ) : Prop
-    := forall e : Γ ⇒ᵥ Δ, (inj_init_act Δ x ∥ inj_init_pas e) ≈ (inj_init_act Δ y ∥ inj_init_pas e).
+    := forall γ : Γ =[val]> Δ,
+         (inj_init_act Δ x ∥ inj_init_pas γ)
+       ≈ (inj_init_act Δ y ∥ inj_init_pas γ).
   Notation "x ≈⟦barb Δ ⟧≈ y" := (barb Δ x y) (at level 50).
 
   Theorem barb_correction {Γ} Δ (x y : conf Γ) : x ≈⟦barb Δ ⟧≈ y -> x ≈⟦ciu Δ ⟧≈ y.
   Proof.
     intros H e.
-    etransitivity; [ apply it_eq_wbisim, (adequacy x e) | ].
-    etransitivity; [ apply iter_evg_iter | ].
-    etransitivity; [ apply (H e) | symmetry ].
-    etransitivity; [ apply it_eq_wbisim, (adequacy y e) | ].
-    etransitivity; [ apply iter_evg_iter | ].
-    reflexivity.
+    rewrite (it_eq_wbisim _ _ _ (adequacy x e)), (it_eq_wbisim _ _ _ (adequacy y e)).
+    unfold compo_ev_guarded; rewrite 2 iter_evg_iter; apply H.
   Qed.
 
   Theorem ogs_correction {Γ} Δ (x y : conf Γ) : x ≈⟦ogs Δ ⟧≈ y -> x ≈⟦ciu Δ ⟧≈ y.
   Proof.
     intro H; apply barb_correction.
     intro e; unfold compo.
-    rewrite <- 2 compo_compo_alt.
+    rewrite <- 2 (compo_compo_alt (x := RedT _ _)).
     apply compo_alt_proper; [ exact H | intro; reflexivity ].
   Qed.
 
-End withFam.
-About ogs_correction.
-Print Assumptions ogs_correction.
+End with_param.
